backend/CleanupLabelsproof.v
@@ -333,12 +333,10 @@ End CLEANUP.
 
 Theorem transf_program_correct prog tprog:
   match_prog prog tprog ->
-  open_fsim cc_id cc_id (Linear.semantics prog) (Linear.semantics tprog).
+  forward_simulation cc_id cc_id (Linear.semantics prog) (Linear.semantics tprog).
 Proof.
-  intros MATCH. split; [apply match_program_skel in MATCH; auto | ].
-  intros [ ] se _ q _ _ _ [ ] [ ].
-  split. { eapply Genv.is_internal_transf_id; eauto. destruct fd; auto. }
-  eapply forward_simulation_opt; simpl.
+  fsim eapply forward_simulation_opt; cbn in *; intros; subst.
+  - apply (Genv.is_internal_transf_id MATCH). intros [|]; auto.
   - eauto using transf_initial_states.
   - eauto using transf_final_states.
   - intros. edestruct transf_external; eauto. exists tt, q1. intuition subst; eauto.
