cfrontend/Cshmgenproof.v
@@ -1776,13 +1776,11 @@ End CORRECTNESS.
 
 Theorem transl_program_correct prog tprog:
   match_prog prog tprog ->
-  open_fsim cc_id cc_id (Clight.semantics2 prog) (Csharpminor.semantics tprog).
+  forward_simulation cc_id cc_id (Clight.semantics2 prog) (Csharpminor.semantics tprog).
 Proof.
-  intros MATCH. split; [apply match_program_skel in MATCH; auto | ].
-  intros [ ] se _ q _ _ _ [ ] [ ].
-  split. { eapply Genv.is_internal_match_id; eauto. destruct 1; auto. }
-  eapply forward_simulation_plus; cbn.
-  - eauto using transl_initial_states.
+  fsim eapply forward_simulation_plus; cbn; destruct w, Hse.
+  - intros q _ [ ]. eapply Genv.is_internal_match_id; eauto. destruct 1; auto.
+  - intros q _ s1 [ ]. eauto using transl_initial_states.
   - eauto using transl_final_states.
   - intros. edestruct transl_external; eauto. exists tt, q1. intuition subst; eauto.
   - eauto using transl_step.
